More progress.

extra/Dijkstra/IterRel.v
@@ -1,7 +1,9 @@
 From Stdlib Require Import Arith Lia.
-From Paco Require Import paco.
+From Coinduction Require Import all. 
 
-From ITree Require Import Axioms.
+From ITree Require Import 
+Axioms
+Utils. 
 
 Create HintDb not_wf.
 
@@ -17,21 +19,18 @@ Section IterRel.
     | not_wf (a' : A) (Hrel : r a a') (Hcorec : F a') .
   Hint Constructors not_wf_F : not_wf.
 
-  Lemma not_wf_F_mono sim sim' a
-        (IN : not_wf_F sim a)
-        (LE : sim <1= sim') : not_wf_F sim' a.
+  Lemma not_wf_F_mono : Proper (leq ==> leq)
+        not_wf_F. 
   Proof.
-    destruct IN. eauto with not_wf.
+    repeat red. intros; inv H0. 
+    econstructor; eauto. now apply H.  
   Qed.
 
-  Lemma not_wf_F_mono' : monotone1 not_wf_F.
-  Proof.
-    red. intros. eapply not_wf_F_mono; eauto.
-  Qed.
-  Hint Resolve not_wf_F_mono' : paco.
+Definition not_wf_F_mon := 
+{| body := not_wf_F ; Hbody := not_wf_F_mono |}.
 
   Definition not_wf_from : A -> Prop :=
-    paco1 not_wf_F bot1.
+    gfp not_wf_F_mon.
 
   Inductive wf_from (a : A) : Prop :=
     | base : (forall a', ~ (r a a')) -> wf_from a
@@ -41,16 +40,16 @@ Section IterRel.
   Lemma neg_wf_from_not_wf_from_l : forall (a : A),
       ~(wf_from a) -> not_wf_from a.
   Proof.
-    pcofix CIH. intros. pfold. destruct (classic (exists a', r a a' /\ ~ ( wf_from a') )).
-    - destruct H as [a' [Hr Hwf] ]. econstructor; eauto.
+    unfold not_wf_from. coinduction c CIH. intros. destruct (classic (exists a', r a a' /\ ~ ( wf_from a') )).
+    - destruct H0 as [a' [Hr Hwf] ]. econstructor; eauto.
     - assert (forall a', ~ r a a' \/ wf_from a').
       {
         intros.
         destruct (classic (r a a')); auto. destruct (classic (wf_from a')); auto.
-        exfalso. apply H. exists a'. auto.
+        exfalso. apply H0. exists a'. auto.
       }
-      clear H.
-      exfalso. apply H0. clear H0. apply step. intros. destruct (H1 a'); auto with not_wf.
+      clear H0.
+      exfalso. apply H. clear H. apply step. intros. destruct (H1 a'); auto with not_wf.
   Qed.
 
   Lemma neg_wf_from_not_wf_from_r : forall (a : A),
